Move lemmas to Lemmas.*.fst

raindrops/Raindrops.fst
@@ -14,24 +14,13 @@ let raindrop n = match of_int n with
             ^ (if n % 5 = 0 then "Plang" else "")
             ^ (if n % 7 = 0 then "Plong" else "")
 
-module S = FStar.String
+module LS = Lemmas.String
 
-val string_of_int_return_not_empty_string: (n:int) -> Lemma (ensures S.length (string_of_int n) <> 0) [SMTPat (string_of_int n)]
-let string_of_int_return_not_empty_string = admit()
-
-val strcat_add_length: (s1:string) -> (s2:string) -> Lemma (ensures (S.length s1) + (S.length s2) = (S.length (s1 ^ s2))) [SMTPat (s1 ^ s2)]
-let strcat_add_length = admit()
-
-val empty_string_length_is_zero: (s:string) -> Lemma (requires s = "") (ensures S.length s = 0)
-let empty_string_length_is_zero = admit()
-
-val not_empty_string_length_is_pos: (s:string) -> Lemma (requires s <> "") (ensures S.length s > 0)
-let not_empty_string_length_is_pos = admit()
-
-val raindrop_return_any_sound: (n:native_int) -> Lemma (ensures S.length (raindrop n) > 0)
-let raindrop_return_any_sound n = match of_int n with
+val raindrop_cause_some_sound: (n:native_int) -> Lemma (raindrop n <> "")
+let raindrop_cause_some_sound n =
+    LS.empty_string_length_is_zero "";
+    match of_int n with
     | n when n % 3 <> 0 && n % 5 <> 0 && n % 7 <> 0 -> ()
-    | n -> empty_string_length_is_zero "";
-            not_empty_string_length_is_pos "Pling";
-            not_empty_string_length_is_pos "Plang";
-            not_empty_string_length_is_pos "Plong"
+    | n -> LS.not_empty_string_length_is_pos "Pling";
+            LS.not_empty_string_length_is_pos "Plang";
+            LS.not_empty_string_length_is_pos "Plong"
